vale/code/arch/x64/interop/new/X64.MemoryAdapters.fst
@@ -1,16 +1,16 @@
 module X64.MemoryAdapters
 
 open Interop.Base
-module B = LowStar.Buffer
-module BS = X64.Bytes_Semantics_s
-module BV = LowStar.BufferView
 module HS = FStar.HyperStack
 module ME = X64.Memory
 module IB = Interop.Base
 module VS = X64.Vale.State
 friend X64.Memory
 module T = FStar.Tactics
-let buffer_eq = assert (ME.buffer == IB.buf_t) by (T.norm [delta_only [`%ME.buffer]]; T.trefl())
+module B = LowStar.Buffer
+
+let as_vale_buffer #t i = IB.Buffer (i <: B.buffer UInt8.t) true
+
 let mem_eq = ()
 let buffer_addr_is_nat64 (#t:_) (x:ME.buffer t) (s:VS.state) = ()
 
