vale/code/arch/x64/interop/new/X64.MemoryAdapters.fsti
@@ -1,7 +1,6 @@
 module X64.MemoryAdapters
 
 open Interop.Base
-module B = LowStar.Buffer
 module BS = X64.Bytes_Semantics_s
 module BV = LowStar.BufferView
 module HS = FStar.HyperStack
@@ -11,17 +10,7 @@ module VS = X64.Vale.State
 module V = X64.Vale.Decls
 module TS = X64.Taint_Semantics_s
 
-val buffer_eq : squash (ME.buffer == IB.buf_t)
-
-unfold
-let as_vale_buffer (#t:_) (i:IB.buf_t t)
-  : ME.buffer t
-  = IB.coerce i
-
-unfold
-let as_lowstar_buffer (#t:_) (i:ME.buffer t)
-  : IB.buf_t t
-  = IB.coerce i
+val as_vale_buffer (#t:_) (i:IB.buf_t t) : ME.buffer t
 
 val mem_eq : squash (ME.mem == IB.mem)
 
